src/RewriterExamples.v
@@ -1,0 +1,87 @@
+Require Import Coq.ZArith.ZArith.
+Require Import Coq.micromega.Lia.
+Require Import Coq.Lists.List.
+Require Import Crypto.RewriterAllTactics.
+Require Import Crypto.IdentifiersGENERATEDProofs.
+Require Import Crypto.PreLanguage.
+Require Import Crypto.Util.LetIn.
+Require Import Crypto.Util.Notations.
+Require Crypto.Util.PrimitiveHList.
+Import ListNotations. Local Open Scope bool_scope. Local Open Scope Z_scope.
+
+Import RewriterAllTactics.Compilers.RewriteRules.GoalType.
+Import RewriterAllTactics.Compilers.RewriteRules.Tactic.
+Import IdentifiersGENERATEDProofs.Compilers.pattern.ident.
+
+Local Notation "' x" := (ident.literal x).
+Local Notation dont_do_again := (pair false) (only parsing).
+Local Notation do_again := (pair true) (only parsing).
+Local Definition mymap {A B} := Eval cbv in @List.map A B.
+Local Definition myapp {A} := Eval cbv in @List.app A.
+
+Definition myruletypes : list (bool * Prop)
+  := Eval cbv [mymap myapp] in
+      myapp
+        (mymap
+           dont_do_again
+           [(forall x, x + 0 = x)
+            ; (forall A B x y, @fst A B (x, y) = x)
+            ; (forall A B x y, @snd A B (x, y) = y)
+            ; (forall A B f ls, @List.map A B f ls
+                                = (ident.eagerly (@list_rect) _ _)
+                                    []
+                                    (fun x xs map_f_xs => f x :: map_f_xs)
+                                    ls)
+            ; (forall A xs ys, @List.app A xs ys
+                               = (ident.eagerly (@list_rect) _ _)
+                                   ys (fun x xs app_xs_ys => x :: app_xs_ys) xs)
+            ; (forall A P N C ls,
+                  @ident.Thunked.list_rect A P N C ls
+                  = ident.eagerly (@ident.Thunked.list_rect) A P N C ls)
+            ; (forall A P Q N C ls v,
+                  @list_rect A (fun _ => P -> Q) N C ls v
+                  = ident.eagerly (@list_rect) A (fun _ => P -> Q) N C ls v)])
+        (mymap
+           do_again
+           [(forall A B f xs,
+                @List.flat_map A B f xs
+                = (list_rect _)
+                    nil
+                    (fun x _ flat_map_tl => f x ++ flat_map_tl)
+                    xs)]).
+
+Lemma myruleproofs
+  : PrimitiveHList.hlist (@snd bool Prop) myruletypes.
+Proof.
+  repeat constructor; cbn [snd]; cbv [ident.eagerly]; intros;
+    try solve [ lia
+              | now apply ListUtil.eq_app_list_rect ].
+Qed.
+
+Definition myrules : VerifiedRewriter.
+Proof using All. make_rewriter package_proofs true myruleproofs. Defined.
+
+Example ex1 : forall x, x + 0 = x.
+Proof.
+  Rewrite_for myrules.
+  lazymatch goal with
+  | |- ?x = ?x => is_var x; reflexivity
+  end.
+Qed.
+
+Ltac test_rewrite :=
+  Rewrite_for myrules;
+  lazymatch goal with
+  | [ |- ?x = ?y ] => first [ constr_eq x y; idtac "Success:" x; reflexivity
+                            | fail 1 x "≢" y ]
+  end.
+
+Example ex2 : forall y e1 e2,
+    map (fun x => y + x) (dlet z := e1 + e2 in [0; 1; 2; z; z+1])
+    = dlet z := e1 + e2 in [y; y + 1; y + 2; y + z; y + (z + 1)].
+Proof. test_rewrite. Qed.
+
+Example ex3 : forall (x1 x2 x3 : Z),
+    flat_map (fun a => [a; a; a]) [x1;x2;x3]
+    = [x1; x1; x1; x2; x2; x2; x3; x3; x3].
+Proof. test_rewrite. Qed.
